Tweaks

src/graph_theory/to_mathlib.lean
@@ -1,7 +1,9 @@
-import combinatorics.simple_graph.basic data.finset.basic
+import combinatorics.simple_graph.connectivity data.finset.basic
+
+variables {V : Type*} {G : simple_graph V}
 
 namespace finset
-@[simp] lemma singleton_inter_nonempty {V : Type*} [decidable_eq V] {a : V} {X : finset V} :
+@[simp] lemma singleton_inter_nonempty [decidable_eq V] {a : V} {X : finset V} :
   ({a} ∩ X).nonempty ↔ a ∈ X :=
 { mp := not_not.mp ∘ mt singleton_inter_of_not_mem ∘ nonempty_iff_ne_empty.mp,
   mpr := eq.rec (singleton_nonempty a) ∘ eq.symm ∘ singleton_inter_of_mem }
@@ -9,4 +11,7 @@ namespace finset
 end finset
 
 namespace simple_graph
+def walk.darts : Π {x y : V}, walk G x y → list G.dart
+| _ _ walk.nil        := []
+| _ _ (walk.cons h p) := ⟨(_,_),h⟩ :: walk.darts p
 end simple_graph
